src/extr.v
@@ -1,0 +1,31 @@
+From Coq Require Extraction ExtrOcamlBasic ExtrOcamlNatInt.
+From mathcomp Require Import ssreflect ssrbool ssrfun.
+From mathcomp Require Import ssrnat seq order eqtype.
+From ipcssr Require Import search.
+
+Set Extraction Flag 522.
+Set Extraction AccessOpaque.
+
+Extract Inlined Constant negb => "not".
+Extract Inlined Constant idP => "".
+
+(* lists *)
+Extract Inlined Constant size => "List.length".
+Extract Inlined Constant cat => "(@)".
+Extract Inlined Constant fst => "fst".
+
+(* ints! *)
+Extract Inlined Constant eqn => "(=)".
+Extract Inlined Constant leq => "(<=)".
+Extract Inlined Constant leqP => "(<=)".
+Extract Inlined Constant ltnP => "(<)".
+Extract Inlined Constant maxn => "Stdlib.max".
+
+Extract Inductive reflect => bool [ true false ].
+Extract Inductive alt_spec => bool [ true false ].
+Extract Inductive leq_xor_gtn => bool [ true false ].
+Extract Inductive ltn_xor_geq => bool [ true false ].
+Extract Inductive eq_xor_neq => bool [ true false ].
+Extract Inductive sum => "Either.t" [ "Either.Left" "Either.Right" ].
+
+Extraction "src/search.ml" search.search.
