theories/weight.v
@@ -1,0 +1,115 @@
+From mathcomp Require Import ssreflect ssrbool ssrfun.
+From mathcomp Require Import ssrnat seq (*bigop*).
+From ipcssr Require Import (*prelude*) forms.
+
+Section Weight.
+Context {A : Type}.
+
+Fixpoint weight (a : form A) : nat :=
+  match a with
+  | Falsum => 1
+  | Atom _ => 1
+  | AndF a b => (weight a + weight b).+1
+  | OrF Falsum b => (weight b).+1
+  | OrF (Atom _) b => (weight b).+1
+  | OrF a b => (weight b + weight a).+2
+  | Imp a b => weight_neg a + weight b
+  end
+with weight_neg (a : form A) : nat :=
+  match a with
+  | Falsum => 0
+  | Atom _ => 0
+  | AndF a b => (weight_neg a + weight_neg b).+1
+  | OrF a b => (weight_neg a + weight_neg b).+3
+  | Imp Falsum b => 1
+  | Imp (Atom _) Falsum => 2
+  | Imp (Atom _) (Atom _) => 1
+  | Imp (Atom _) b => (weight_neg b).+3
+  | Imp a b => (weight_neg b + weight a).+4
+  end.
+
+Fixpoint weight_goal (a : form A) : nat :=
+  match a with
+  | Falsum => 0
+  | Atom _ => 0
+  | AndF _ _ => 1
+  | OrF _ _ => 1
+  | Imp _ b => (weight_goal b).+1
+  end.
+
+Definition weight_gamma :=
+  foldr (fun a n => weight a + n) 0.
+
+(*
+Lemma weight_gammaE l :
+  weight_gamma l = \sum_(i <- l) weight i.
+Proof. by rewrite /weight_gamma -fusion_map foldrE big_map. Qed.
+*)
+
+(**********************************************************************)
+
+Lemma weight_ge_1 a : 0 < weight a.
+Proof.
+elim: a=>//=; first by case.
+move=>f1 H1 f2 H2.
+by apply: ltn_addl.
+Qed.
+
+Lemma weight_neg_le j a :
+ weight_neg (Imp (Atom j) a) <= (weight_neg a).+3.
+Proof. by case: a. Qed.
+
+Lemma weight_vimp l a : weight (vimp l a) = weight a.
+Proof.
+elim: l a=>//= x l IH a.
+by apply: (IH (Imp (Atom x) a)).
+Qed.
+
+Lemma weight_gamma_weak a b gamma n :
+  weight a < weight b ->
+  weight_gamma (b :: gamma) <= n ->
+  weight_gamma (a :: gamma) < n.
+Proof.
+move=>/= H Hb.
+apply/leq_trans/Hb.
+by rewrite ltn_add2r.
+Qed.
+
+Lemma weight_gamma_weak' a b gamma n :
+  weight a < weight b ->
+  weight b + weight_gamma gamma <= n ->
+  weight a + weight_gamma gamma < n.
+Proof. by apply: weight_gamma_weak. Qed.
+
+Lemma weight_gamma_weak2 a b c gamma n :
+  weight a + weight b < weight c ->
+  weight_gamma (c :: gamma) <= n -> weight_gamma (a :: b :: gamma) < n.
+Proof.
+move=>/= H Hac.
+apply/leq_trans/Hac.
+by rewrite addnA ltn_add2r.
+Qed.
+
+Lemma weight_gamma_weak2' a b c gamma n :
+  weight a + weight b < weight c ->
+  weight c + weight_gamma gamma <= n ->
+  weight a + (weight b + weight_gamma gamma) < n.
+Proof. by apply: weight_gamma_weak2. Qed.
+
+Lemma weight_gamma_weak3 a b c d gamma n :
+  weight a + weight b + weight c < weight d ->
+  weight_gamma (d :: gamma) <= n ->
+  weight_gamma (a :: b :: c :: gamma) < n.
+Proof.
+move=>/= H Hd.
+apply/leq_trans/Hd.
+by rewrite !addnA ltn_add2r.
+Qed.
+
+Lemma weight_gamma_weak3' a b c d gamma n :
+  weight a + weight b + weight c < weight d ->
+  weight d + weight_gamma gamma <= n ->
+  weight a + (weight b + (weight c + weight_gamma gamma)) < n.
+Proof. by apply: weight_gamma_weak3. Qed.
+
+End Weight.
